Lambda/InductTermi made new-style theory; tuned;

src/HOL/Lambda/InductTermi.thy
@@ -9,14 +9,108 @@ Raamsdonk & Severi. On normalization. CWI TR CS-R9545, 1995.
 Also rediscovered by Matthes and Joachimski.
 *)
 
-InductTermi = ListBeta +
+theory InductTermi = ListBeta:
 
-consts IT :: dB set
+consts
+  IT :: "dB set"
+
 inductive IT
-intrs
-VarI "rs : lists IT ==> (Var n)$$rs : IT"
-LambdaI "r : IT ==> Abs r : IT"
-BetaI "[| (r[s/0])$$ss : IT; s : IT |] ==> (Abs r $ s)$$ss : IT"
-monos lists_mono
+  intros
+    Var: "rs : lists IT ==> Var n $$ rs : IT"
+    Lambda: "r : IT ==> Abs r : IT"
+    Beta: "[| (r[s/0])$$ss : IT; s : IT |] ==> (Abs r $ s)$$ss : IT"
+  monos lists_mono       (* FIXME move to HOL!? *)
+
+
+text {* Every term in IT terminates. *}
+
+lemma double_induction_lemma [rulify]:
+  "s : termi beta ==> \<forall>t. t : termi beta -->
+    (\<forall>r ss. t = r[s/0] $$ ss --> Abs r $ s $$ ss : termi beta)"
+  apply (erule acc_induct)
+  apply (erule thin_rl)
+  apply (rule allI)
+  apply (rule impI)
+  apply (erule acc_induct)
+  apply clarify
+  apply (rule accI)
+  apply (tactic {* safe_tac (claset () addSEs [apps_betasE]) *})  -- FIXME
+     apply assumption
+    apply (blast intro: subst_preserves_beta apps_preserves_beta)
+   apply (blast intro: apps_preserves_beta2 subst_preserves_beta2 rtrancl_converseI
+     dest: acc_downwards)  (* FIXME: acc_downwards can be replaced by acc(R ^* ) = acc(r) *)
+  apply (blast dest: apps_preserves_betas)
+  done
+
+lemma IT_implies_termi: "t : IT ==> t : termi beta"
+  apply (erule IT.induct)
+    apply (drule rev_subsetD)
+     apply (rule lists_mono)
+     apply (rule Int_lower2)
+    apply simp
+    apply (drule lists_accD)
+    apply (erule acc_induct)
+    apply (rule accI)
+    apply (blast dest: head_Var_reduction)
+   apply (erule acc_induct)
+   apply (rule accI)
+   apply blast
+  apply (blast intro: double_induction_lemma)
+  done
+
+
+text {* Every terminating term is in IT *}
+
+declare Var_apps_neq_Abs_apps [THEN not_sym, simp]
+
+lemma [simp, THEN not_sym, simp]: "Var n $$ ss ~= Abs r $ s $$ ts"
+  apply (simp add: foldl_Cons [symmetric] del: foldl_Cons)
+  done
+
+lemma [simp]:
+  "(Abs r $ s $$ ss = Abs r' $ s' $$ ss') = (r=r' \<and> s=s' \<and> ss=ss')"
+  apply (simp add: foldl_Cons [symmetric] del: foldl_Cons)
+  done
+
+inductive_cases [elim!]:
+  "Var n $$ ss : IT"
+  "Abs t : IT"
+  "Abs r $ s $$ ts : IT"
+
+
+theorem termi_implies_IT: "r : termi beta ==> r : IT"
+  apply (erule acc_induct)
+  apply (rename_tac r)
+  apply (erule thin_rl)
+  apply (erule rev_mp)
+  apply simp
+  apply (rule_tac t = r in Apps_dB_induct)
+   apply clarify
+   apply (rule IT.intros)
+   apply clarify
+   apply (drule bspec, assumption)
+   apply (erule mp)
+   apply clarify
+   apply (drule converseI)
+   apply (drule ex_step1I, assumption)
+   apply clarify
+   apply (rename_tac us)
+   apply (erule_tac x = "Var n $$ us" in allE)
+   apply force
+   apply (rename_tac u ts)
+   apply (case_tac ts)
+    apply simp
+    apply (blast intro: IT.intros)
+   apply (rename_tac s ss)
+   apply simp
+   apply clarify
+   apply (rule IT.intros)
+    apply (blast intro: apps_preserves_beta)
+   apply (erule mp)
+   apply clarify
+   apply (rename_tac t)
+   apply (erule_tac x = "Abs u $ t $$ ss" in allE)
+   apply force
+   done
 
 end
